Tests/STLC_Eval/TrmSpec.lean
@@ -11,7 +11,7 @@ open Tests.STLC_Eval.Sanity.Symbolic
 namespace Fixture
 
 @[reducible] unsafe def _unsafeFBoundGroup (T : Type) :
-    FBoundGroup I.Index T :=
+    FBound I.Index T :=
   let saved : IO.Ref (Array T) := unsafeBaseIO (IO.mkRef #[])
   let save : T → I.Index := fun value =>
     unsafeBaseIO do
